theories/logic/proofmode/spec_tactics.v
@@ -10,10 +10,10 @@ Set Default Proof Using "Type".
 (** * TP tactics *)
 
 (** ** bind *)
-Lemma tac_tp_bind_gen `{relocG Σ} j Δ Δ' i p e e' Q :
-  envs_lookup i Δ = Some (p, j ⤇ e)%I →
+Lemma tac_tp_bind_gen `{relocG Σ} k Δ Δ' i p e e' Q :
+  envs_lookup i Δ = Some (p, refines_right k e)%I →
   e = e' →
-  envs_simple_replace i p (Esnoc Enil i (j ⤇ e')) Δ = Some Δ' →
+  envs_simple_replace i p (Esnoc Enil i (refines_right k e')) Δ = Some Δ' →
   (envs_entails Δ' Q) →
   (envs_entails Δ Q).
 Proof.
@@ -22,10 +22,10 @@ Proof.
   destruct p; rewrite /= ?right_id; by rewrite bi.wand_elim_r.
 Qed.
 
-Lemma tac_tp_bind `{relocG Σ} j e' Δ Δ' i p K' e Q :
-  envs_lookup i Δ = Some (p, j ⤇ e)%I →
+Lemma tac_tp_bind `{relocG Σ} k e' Δ Δ' i p K' e Q :
+  envs_lookup i Δ = Some (p, refines_right k e)%I →
   e = fill K' e' →
-  envs_simple_replace i p (Esnoc Enil i (j ⤇ fill K' e')) Δ = Some Δ' →
+  envs_simple_replace i p (Esnoc Enil i (refines_right k (fill K' e'))) Δ = Some Δ' →
   (envs_entails Δ' Q) →
   (envs_entails Δ Q).
 Proof. intros. by eapply tac_tp_bind_gen. Qed.
@@ -64,7 +64,7 @@ Tactic Notation "tp_bind" constr(j) open_constr(efoc) :=
     |reflexivity
     |(* new goal *)].
 
-Lemma tac_tp_pure `{relocG Σ} e K' e1 j e2 Δ1 E1 i1 i2 p e' ϕ ψ Q n :
+Lemma tac_tp_pure `{relocG Σ} e K' e1 k e2 Δ1 E1 i1 e' ϕ ψ Q n :
   (* we have those premises first, because we will be trying to solve them
      with backtracking using reashape_expr; see the accompanying Ltac.
      the first premise decomposes the expression, the second one checks
@@ -73,32 +73,32 @@ Lemma tac_tp_pure `{relocG Σ} e K' e1 j e2 Δ1 E1 i1 i2 p e' ϕ ψ Q n :
   PureExec ϕ n e1 e2 →
   (∀ P, ElimModal ψ false false (|={E1}=> P) P Q Q) →
   nclose specN ⊆ E1 →
-  envs_lookup i1 Δ1 = Some (p, spec_ctx) →
-  envs_lookup i2 Δ1 = Some (false, j ⤇ e)%I →
+  envs_lookup i1 Δ1 = Some (false, refines_right k e)%I →
   ψ →
   ϕ →
   (* we will call simpl on this goal thus re-composing the expression again *)
   e' = fill K' e2 →
-  match envs_simple_replace i2 false (Esnoc Enil i2 (j ⤇ e')) Δ1 with
+  match envs_simple_replace i1 false (Esnoc Enil i1 (refines_right k e')) Δ1 with
   | Some Δ2 => envs_entails Δ2 Q
   | None => False
   end →
   envs_entails Δ1 Q.
 Proof.
-  rewrite envs_entails_eq. intros -> Hpure ?? HΔ1 ? Hψ Hϕ -> ?.
-  rewrite -(idemp bi_and (of_envs Δ1)).
-  rewrite {1}(envs_lookup_sound' Δ1 false). 2: apply HΔ1.
-  rewrite bi.sep_elim_l.
-  enough (<pers> spec_ctx ∧ of_envs Δ1 -∗ Q) as <-.
-  { rewrite -bi.intuitionistically_into_persistently_1.
-    destruct p; simpl;
-    by rewrite ?(bi.intuitionistic_intuitionistically spec_ctx). }
-  rewrite bi.persistently_and_intuitionistically_sep_l.
-  rewrite bi.intuitionistic_intuitionistically.
+  rewrite envs_entails_eq. intros -> Hpure ?? HΔ1 Hψ Hϕ -> ?.
+  (* rewrite -(idemp bi_and (of_envs Δ1)). *)
+  (* rewrite {1}(envs_lookup_sound' Δ1 false). 2: apply HΔ1. *)
+  (* rewrite bi.sep_elim_l. *)
+  (* enough (<pers> spec_ctx ∧ of_envs Δ1 -∗ Q) as <-. *)
+  (* { rewrite -bi.intuitionistically_into_persistently_1. *)
+  (*   destruct p; simpl; *)
+  (*   by rewrite ?(bi.intuitionistic_intuitionistically spec_ctx). } *)
+  (* rewrite bi.persistently_and_intuitionistically_sep_l. *)
+  (* rewrite bi.intuitionistic_intuitionistically. *)
   destruct (envs_simple_replace _ _ _ _) as [Δ2|] eqn:HΔ2; try done.
-  rewrite (envs_simple_replace_sound Δ1 Δ2 i2) //; simpl.
+  rewrite (envs_simple_replace_sound Δ1 Δ2 i1) //; simpl.
   rewrite right_id.
-  rewrite (assoc _ spec_ctx (j ⤇ _)%I).
+  rewrite /refines_right.
+  (* rewrite (assoc _ spec_ctx (j ⤇ _)%I). *)
   rewrite step_pure //.
   rewrite -[Q]elim_modal // /=.
   apply bi.sep_mono_r.
@@ -106,40 +106,28 @@ Proof.
   by rewrite bi.wand_elim_r.
 Qed.
 
-(* helper tactic allowing us to use tp_ tactics whenever our goal is a refinement *)
-Ltac with_spec_ctx tac :=
-  lazymatch goal with
-  | |- envs_entails _ (refines ?E ?e1 ?e2 ?A) =>
-    let H := iFresh in
-    iApply (refines_spec_ctx E e1 e2 A);
-    iIntros H;
-    (tac (); iClear H)
-  | _ => tac ()
-  end.
-
 Tactic Notation "tp_pure" constr(j) open_constr(ef) :=
   iStartProof;
-  with_spec_ctx ltac:(fun _ =>
-      lazymatch goal with
-      | |- context[environments.Esnoc _ ?H (j ⤇ fill ?K' ?e)] =>
-        reshape_expr e ltac:(fun K e' =>
-            unify e' ef;
-            eapply (tac_tp_pure (fill K' e) (K++K') e' j);
-            [by rewrite ?fill_app | iSolveTC | ..])
-      | |- context[environments.Esnoc _ ?H (j ⤇ ?e)] =>
-        reshape_expr e ltac:(fun K e' =>
-            unify e' ef;
-            eapply (tac_tp_pure e K e' j);
-            [by rewrite ?fill_app | iSolveTC | ..])
-      end;
-      [iSolveTC || fail "tp_pure: cannot eliminate modality in the goal"
-      |solve_ndisj || fail "tp_pure: cannot prove 'nclose specN ⊆ ?'"
-      |iAssumptionCore || fail "tp_pure: cannot find spec_ctx" (* spec_ctx *)
-      |iAssumptionCore || fail "tp_pure: cannot find '" j " ⤇ ?'"
-      |try (exact I || reflexivity) (* ψ *)
-      |try (exact I || reflexivity) (* ϕ *)
-      |simpl; reflexivity ||  fail "tp_pure: this should not happen" (* e' = fill K' e2 *)
-      |pm_reduce (* new goal *)]).
+  lazymatch goal with
+  | |- context[environments.Esnoc _ ?H (refines_right j (fill ?K' ?e))] =>
+    reshape_expr e ltac:(fun K e' =>
+      unify e' ef;
+      eapply (tac_tp_pure (fill K' e) (K++K') e' j);
+      [by rewrite ?fill_app | iSolveTC | ..])
+  | |- context[environments.Esnoc _ ?H (refines_right j ?e)] =>
+    reshape_expr e ltac:(fun K e' =>
+      unify e' ef;
+      eapply (tac_tp_pure e K e' j);
+      [by rewrite ?fill_app | iSolveTC | ..])
+  end;
+  [iSolveTC || fail "tp_pure: cannot eliminate modality in the goal"
+  |solve_ndisj || fail "tp_pure: cannot prove 'nclose specN ⊆ ?'"
+  (* |iAssumptionCore || fail "tp_pure: cannot find spec_ctx" (* spec_ctx *) *)
+  |iAssumptionCore || fail "tp_pure: cannot find the RHS" (* TODO fix error message *)
+  |try (exact I || reflexivity) (* ψ *)
+  |try (exact I || reflexivity) (* ϕ *)
+  |simpl; reflexivity ||  fail "tp_pure: this should not happen" (* e' = fill K' e2 *)
+  |pm_reduce (* new goal *)].
 
 
 Tactic Notation "tp_pures" constr (j) := repeat (tp_pure j _).
@@ -165,174 +153,145 @@ Tactic Notation "tp_if" constr(j) := tp_pure j (If _ _ _).
 Tactic Notation "tp_pair" constr(j) := tp_pure j (Pair _ _).
 Tactic Notation "tp_closure" constr(j) := tp_pure j (Rec _ _ _).
 
-Lemma tac_tp_store `{relocG Σ} j Δ1 Δ2 E1 i1 i2 i3 p K' e (l : loc) e' e2 v' v Q :
+Lemma tac_tp_store `{relocG Σ} k Δ1 Δ2 E1 i1 i2 K' e (l : loc) e' e2 v' v Q :
   (* TODO: here instead of True we can consider another Coq premise, like in tp_pure.
      Same goes for the rest of those tactics *)
   (∀ P, ElimModal True false false (|={E1}=> P) P Q Q) →
   nclose specN ⊆ E1 →
-  envs_lookup i1 Δ1 = Some (p, spec_ctx) →
-  envs_lookup_delete false i2 Δ1 = Some (false, j ⤇ e, Δ2)%I →
+  envs_lookup_delete false i1 Δ1 = Some (false, refines_right k e, Δ2)%I →
   e = fill K' (Store (# l) e') →
   IntoVal e' v →
   (* re-compose the expression and the evaluation context *)
   e2 = fill K' #() →
-  envs_lookup i3 Δ2 = Some (false, l ↦ₛ v')%I →
-  match envs_simple_replace i3 false
-     (Esnoc (Esnoc Enil i2 (j ⤇ e2)) i3 (l ↦ₛ v)) Δ2 with
+  envs_lookup i2 Δ2 = Some (false, l ↦ₛ v')%I →
+  match envs_simple_replace i2 false
+     (Esnoc (Esnoc Enil i1 (refines_right k e2)) i2 (l ↦ₛ v)) Δ2 with
   | None => False
   | Some Δ3 => envs_entails Δ3 Q
   end →
   envs_entails Δ1 Q.
 Proof.
-  rewrite envs_entails_eq. intros ???? -> <- -> ? HQ.
-  rewrite -(idemp bi_and (of_envs Δ1)).
-  rewrite {1}(envs_lookup_sound' _ false). 2: eassumption.
-  rewrite bi.sep_elim_l.
-  enough (spec_ctx ∗ of_envs Δ1 -∗ Q) as Hq.
-  { rewrite -Hq.
-    destruct p; simpl; last rewrite -(bi.intuitionistic_intuitionistically spec_ctx);
-    rewrite {1}bi.intuitionistically_into_persistently_1 bi.persistently_and_intuitionistically_sep_l;
-    by rewrite (bi.intuitionistic_intuitionistically spec_ctx). }
+  rewrite /IntoVal.
+  rewrite envs_entails_eq. intros ??? -> <- -> ? HQ.
   rewrite envs_lookup_delete_sound //; simpl.
   destruct (envs_simple_replace _ _ _ _) as [Δ3|] eqn:HΔ3; last done.
   rewrite envs_simple_replace_sound //; simpl.
   rewrite right_id.
   rewrite !assoc -(assoc _ spec_ctx).
-  rewrite step_store //.
+  rewrite -fill_app step_store // fill_app.
   rewrite -[Q]elim_modal //.
   apply bi.sep_mono_r.
   apply bi.wand_intro_l.
-  rewrite (comm _ _ (l ↦ₛ v)%I).
+  rewrite (comm _ _ (l ↦ₛ v)%I). simpl.
+  rewrite assoc. rewrite (comm _ spec_ctx (l ↦ₛ _)%I).
   by rewrite bi.wand_elim_r.
 Qed.
 
 Tactic Notation "tp_store" constr(j) :=
   iStartProof;
-  with_spec_ctx ltac:(fun _ =>
-      eapply (tac_tp_store j);
-        [iSolveTC || fail "tp_store: cannot eliminate modality in the goal"
-        |solve_ndisj || fail "tp_store: cannot prove 'nclose specN ⊆ ?'"
-        |iAssumptionCore || fail "tp_store: cannot find spec_ctx" (* spec_ctx *)
-        |iAssumptionCore || fail "tp_store: cannot find '" j " ⤇ ?'"
-        |tp_bind_helper
-        |iSolveTC || fail "tp_store: cannot convert the argument to a value"
-        |simpl; reflexivity || fail "tp_store: this should not happen"
-        |iAssumptionCore || fail "tp_store: cannot find '? ↦ₛ ?'"
-        |pm_reduce (* new goal *)]).
+  eapply (tac_tp_store j);
+  [iSolveTC || fail "tp_store: cannot eliminate modality in the goal"
+  |solve_ndisj || fail "tp_store: cannot prove 'nclose specN ⊆ ?'"
+  |iAssumptionCore || fail "tp_store: cannot find '" j " ' RHS"
+  |tp_bind_helper
+  |iSolveTC || fail "tp_store: cannot convert the argument to a value"
+  |simpl; reflexivity || fail "tp_store: this should not happen"
+  |iAssumptionCore || fail "tp_store: cannot find '? ↦ₛ ?'"
+  |pm_reduce (* new goal *)].
 
-(*
-DF:
-If [envs_lookup i1 Δ1 = Some (p, spec_ctx ρ)] and
-   [envs_lookup i2 Δ1 = Some (false, j ⤇ fill K e)],
-how can we prove that [i1 <> i2]? If we can do that then we can utilize
-the lemma [envs_lookup_envs_delete_ne].
-*)
+(* *)
+(* DF: *)
+(* If [envs_lookup i1 Δ1 = Some (p, spec_ctx ρ)] and *)
+(*    [envs_lookup i2 Δ1 = Some (false, j ⤇ fill K e)], *)
+(* how can we prove that [i1 <> i2]? If we can do that then we can utilize *)
+(* the lemma [envs_lookup_envs_delete_ne]. *)
+(* *)
 
-Lemma tac_tp_load `{relocG Σ} j Δ1 Δ2 E1 i1 i2 i3 p K' e e2 (l : loc) v Q q :
+Lemma tac_tp_load `{relocG Σ} k Δ1 Δ2 E1 i1 i2 K' e e2 (l : loc) v Q q :
   (∀ P, ElimModal True false false (|={E1}=> P) P Q Q) →
   nclose specN ⊆ E1 →
-  envs_lookup i1 Δ1 = Some (p, spec_ctx) →
-  envs_lookup_delete false i2 Δ1 = Some (false, j ⤇ e, Δ2)%I →
+  envs_lookup_delete false i1 Δ1 = Some (false, refines_right k e, Δ2)%I →
   e = fill K' (Load #l) →
-  envs_lookup i3 Δ2 = Some (false, l ↦ₛ{q} v)%I →
+  envs_lookup i2 Δ2 = Some (false, l ↦ₛ{q} v)%I →
   e2 = fill K' (of_val v) →
-  match envs_simple_replace i3 false
-    (Esnoc (Esnoc Enil i2 (j ⤇ e2)) i3 (l ↦ₛ{q} v)%I) Δ2 with
+  match envs_simple_replace i2 false
+    (Esnoc (Esnoc Enil i1 (refines_right k e2)) i2 (l ↦ₛ{q} v)%I) Δ2 with
   | Some Δ3 => envs_entails Δ3 Q
   | None    => False
   end →
   envs_entails Δ1 Q.
 Proof.
-  rewrite envs_entails_eq. intros ???? -> ? -> HQ.
-  rewrite -(idemp bi_and (of_envs Δ1)).
-  rewrite {1}(envs_lookup_sound' Δ1 false); last by eassumption.
-  rewrite bi.sep_elim_l.
-  enough (spec_ctx ∗ of_envs Δ1 -∗ Q) as Hq.
-  { rewrite -Hq.
-    destruct p; simpl; last rewrite -(bi.intuitionistic_intuitionistically spec_ctx);
-    rewrite {1}bi.intuitionistically_into_persistently_1 bi.persistently_and_intuitionistically_sep_l;
-    by rewrite (bi.intuitionistic_intuitionistically spec_ctx). }
+  rewrite envs_entails_eq. intros ??? -> ? -> HQ.
   rewrite envs_lookup_delete_sound //; simpl.
   destruct (envs_simple_replace _ _ _ _) as [Δ3|] eqn:HΔ3; last done.
-  rewrite (envs_simple_replace_sound Δ2 Δ3 i3) //; simpl.
+  rewrite (envs_simple_replace_sound Δ2 Δ3 i2) //; simpl.
+  rewrite /refines_right.
   rewrite right_id.
-  rewrite (assoc _ spec_ctx (j ⤇ fill K' (Load _))%I).
-  rewrite assoc.
-  rewrite -(assoc _ spec_ctx (j ⤇ fill K' (Load _))%I).
-  rewrite step_load //.
+  rewrite assoc. rewrite -(assoc _ spec_ctx).
+  rewrite -fill_app step_load /= // fill_app.
   rewrite -[Q]elim_modal //.
   apply bi.sep_mono_r.
   apply bi.wand_intro_l.
   rewrite (comm _ _ (l ↦ₛ{q} v)%I).
+  rewrite assoc.
+  rewrite (comm _ _ (l ↦ₛ{q} v)%I).
+  rewrite -assoc.
   rewrite HQ. by apply bi.wand_elim_r.
 Qed.
 
 Tactic Notation "tp_load" constr(j) :=
   iStartProof;
-  with_spec_ctx ltac:(fun _ =>
-      eapply (tac_tp_load j);
-        [iSolveTC || fail "tp_load: cannot eliminate modality in the goal"
-        |solve_ndisj || fail "tp_load: cannot prove 'nclose specN ⊆ ?'"
-        |iAssumptionCore || fail "tp_load: cannot find spec_ctx" (* spec_ctx *)
-        |iAssumptionCore || fail "tp_load: cannot find '" j " ⤇ ?'"
-        |tp_bind_helper
-        |iAssumptionCore || fail "tp_load: cannot find '? ↦ₛ ?'"
-        |simpl; reflexivity || fail "tp_load: this should not happen"
-        |pm_reduce (* new goal *)]).
+  eapply (tac_tp_load j);
+  [iSolveTC || fail "tp_load: cannot eliminate modality in the goal"
+  |solve_ndisj || fail "tp_load: cannot prove 'nclose specN ⊆ ?'"
+  |iAssumptionCore || fail "tp_load: cannot find the RHS '" j "'"
+  |tp_bind_helper
+  |iAssumptionCore || fail "tp_load: cannot find '? ↦ₛ ?'"
+  |simpl; reflexivity || fail "tp_load: this should not happen"
+  |pm_reduce (* new goal *)].
 
-Lemma tac_tp_cmpxchg_fail `{relocG Σ} j Δ1 Δ2 E1 i1 i2 i3 p K' e enew (l : loc) e1 e2 v' v1 v2 Q q :
+Lemma tac_tp_cmpxchg_fail `{relocG Σ} k Δ1 Δ2 E1 i1 i2 K' e enew (l : loc) e1 e2 v' v1 v2 Q q :
   (∀ P, ElimModal True false false (|={E1}=> P) P Q Q) →
   nclose specN ⊆ E1 →
-  envs_lookup i1 Δ1 = Some (p, spec_ctx) →
-  envs_lookup_delete false i2 Δ1 = Some (false, j ⤇ e, Δ2)%I →
+  envs_lookup_delete false i1 Δ1 = Some (false, refines_right k e, Δ2)%I →
   e = fill K' (CmpXchg #l e1 e2) →
   IntoVal e1 v1 →
   IntoVal e2 v2 →
-  envs_lookup i3 Δ2 = Some (false, l ↦ₛ{q} v')%I →
+  envs_lookup i2 Δ2 = Some (false, l ↦ₛ{q} v')%I →
   v' ≠ v1 →
   vals_compare_safe v' v1 →
   enew = fill K' (v', #false)%V →
-  match envs_simple_replace i3 false
-    (Esnoc (Esnoc Enil i2 (j ⤇ enew)) i3 (l ↦ₛ{q} v')%I) Δ2 with
+  match envs_simple_replace i2 false
+    (Esnoc (Esnoc Enil i1 (refines_right k enew)) i2 (l ↦ₛ{q} v')%I) Δ2 with
   | Some Δ3 => envs_entails Δ3 Q
   | None    =>  False
   end →
   envs_entails Δ1 Q.
 Proof.
-  rewrite envs_entails_eq. intros ???? -> Hv1 Hv2 ??? -> HQ.
-  rewrite -(idemp bi_and (of_envs Δ1)).
-  rewrite {1}(envs_lookup_sound' Δ1 false); last by eassumption.
-  rewrite bi.sep_elim_l.
-  enough (spec_ctx ∗ of_envs Δ1 -∗ Q) as Hq.
-  { rewrite -Hq.
-    destruct p; simpl; last rewrite -(bi.intuitionistic_intuitionistically spec_ctx);
-    rewrite {1}bi.intuitionistically_into_persistently_1 bi.persistently_and_intuitionistically_sep_l;
-    by rewrite (bi.intuitionistic_intuitionistically spec_ctx). }
+  rewrite envs_entails_eq. intros ??? -> Hv1 Hv2 ??? -> HQ.
   rewrite envs_lookup_delete_sound //; simpl.
   destruct (envs_simple_replace _ _ _ _) as [Δ3|] eqn:HΔ3; last done.
-  rewrite (envs_simple_replace_sound Δ2 Δ3 i3) //; simpl.
+  rewrite (envs_simple_replace_sound Δ2 Δ3 i2) //; simpl.
   rewrite right_id.
-  (* (S spec_ctx (S (j => fill _ _) (S (l ↦ v) ..))) *)
-  rewrite (assoc _ spec_ctx (j ⤇ fill K' _)%I).
-  (* (S (S spec_ctx (j => fill _ _)) (S (l ↦ v) ..)) *)
-  rewrite assoc.
-  rewrite -(assoc _ spec_ctx (j ⤇ fill K' _)%I).
-  rewrite step_cmpxchg_fail //.
+  rewrite /refines_right. rewrite -fill_app.
+  rewrite assoc. rewrite -(assoc _ spec_ctx).
+  rewrite step_cmpxchg_fail //. rewrite fill_app.
   rewrite -[Q]elim_modal //.
   apply bi.sep_mono_r.
   apply bi.wand_intro_l.
   rewrite (comm _ _ (l ↦ₛ{q} _)%I).
+  rewrite assoc.
+  rewrite (comm _ _ (l ↦ₛ{q} _)%I).
+  rewrite -assoc.
   rewrite HQ. by apply bi.wand_elim_r.
 Qed.
 
 Tactic Notation "tp_cmpxchg_fail" constr(j) :=
   iStartProof;
-  with_spec_ctx ltac:(fun _ =>
   eapply (tac_tp_cmpxchg_fail j);
     [iSolveTC || fail "tp_cmpxchg_fail: cannot eliminate modality in the goal"
     |solve_ndisj || fail "tp_cmpxchg_fail: cannot prove 'nclose specN ⊆ ?'"
-    |iAssumptionCore || fail "tp_cmpxchg_fail: cannot find spec_ctx" (* spec_ctx *)
-    |iAssumptionCore || fail "tp_cmpxchg_fail: cannot find '" j " ⤇ ?'"
+    |iAssumptionCore || fail "tp_cmpxchg_fail: cannot find the RHS '" j "'"
     |tp_bind_helper (* e = K'[CmpXchg _ _ _] *)
     |iSolveTC || fail "tp_cmpxchg_fail: argument is not a value"
     |iSolveTC || fail "tp_cmpxchg_fail: argument is not a value"
@@ -340,234 +299,191 @@ Tactic Notation "tp_cmpxchg_fail" constr(j) :=
     |try (simpl; congruence) (* v' ≠ v1 *)
     |try heap_lang.proofmode.solve_vals_compare_safe
     |simpl; reflexivity || fail "tp_cmpxchg_fail: this should not happen"
-    |pm_reduce (* new goal *)]).
+    |pm_reduce (* new goal *)].
 
-Lemma tac_tp_cmpxchg_suc `{relocG Σ} j Δ1 Δ2 E1 i1 i2 i3 p K' e enew (l : loc) e1 e2 v' v1 v2 Q :
+Lemma tac_tp_cmpxchg_suc `{relocG Σ} k Δ1 Δ2 E1 i1 i2 K' e enew (l : loc) e1 e2 v' v1 v2 Q :
   (∀ P, ElimModal True false false (|={E1}=> P) P Q Q) →
   nclose specN ⊆ E1 →
-  envs_lookup i1 Δ1 = Some (p, spec_ctx) →
-  envs_lookup_delete false i2 Δ1 = Some (false, j ⤇ e, Δ2)%I →
+  envs_lookup_delete false i1 Δ1 = Some (false, refines_right k e, Δ2)%I →
   e = fill K' (CmpXchg #l e1 e2) →
   IntoVal e1 v1 →
   IntoVal e2 v2 →
-  envs_lookup i3 Δ2 = Some (false, l ↦ₛ v')%I →
+  envs_lookup i2 Δ2 = Some (false, l ↦ₛ v')%I →
   v' = v1 →
   vals_compare_safe v' v1 →
   enew = fill K' (v', #true)%V →
-  match envs_simple_replace i3 false
-    (Esnoc (Esnoc Enil i2 (j ⤇ enew)) i3 (l ↦ₛ v2)%I) Δ2 with
+  match envs_simple_replace i2 false
+    (Esnoc (Esnoc Enil i1 (refines_right k enew)) i2 (l ↦ₛ v2)%I) Δ2 with
   | Some Δ3 => envs_entails Δ3 Q
   | None => False
   end →
   envs_entails Δ1 Q.
 Proof.
-  rewrite envs_entails_eq. intros ???? -> Hv1 Hv2 ??? -> HQ.
-  rewrite -(idemp bi_and (of_envs Δ1)).
-  rewrite {1}(envs_lookup_sound' Δ1 false); last by eassumption.
-  rewrite bi.sep_elim_l.
-  enough (spec_ctx ∗ of_envs Δ1 -∗ Q) as Hq.
-  { rewrite -Hq.
-    destruct p; simpl; last rewrite -(bi.intuitionistic_intuitionistically spec_ctx);
-    rewrite {1}bi.intuitionistically_into_persistently_1 bi.persistently_and_intuitionistically_sep_l;
-    by rewrite (bi.intuitionistic_intuitionistically spec_ctx). }
+  rewrite envs_entails_eq. intros ??? -> Hv1 Hv2 ??? -> HQ.
   rewrite envs_lookup_delete_sound //; simpl.
   destruct (envs_simple_replace _ _ _ _) as [Δ3|] eqn:HΔ3; last done.
-  rewrite (envs_simple_replace_sound Δ2 Δ3 i3) //; simpl.
+  rewrite (envs_simple_replace_sound Δ2 Δ3 i2) //; simpl.
   rewrite right_id.
-  (* (S spec_ctx (S (j => fill _ _) (S (l ↦ v) ..))) *)
-  rewrite (assoc _ spec_ctx (j ⤇ fill K' _)%I).
-  (* (S (S spec_ctx (j => fill _ _)) (S (l ↦ v) ..)) *)
-  rewrite assoc.
-  rewrite -(assoc _ spec_ctx (j ⤇ fill K' _)%I).
-  rewrite step_cmpxchg_suc //.
+  rewrite /refines_right. rewrite -fill_app.
+  rewrite assoc. rewrite -(assoc _ spec_ctx).
+  rewrite step_cmpxchg_suc //. rewrite fill_app.
   rewrite -[Q]elim_modal //.
   apply bi.sep_mono_r.
   apply bi.wand_intro_l.
-  rewrite (comm _ _ (l ↦ₛ _)%I).
+  rewrite (comm _ _ (l ↦ₛ _)%I) assoc.
+  rewrite (comm _ _ (l ↦ₛ _)%I) -assoc.
   rewrite HQ. by apply bi.wand_elim_r.
 Qed.
 
 Tactic Notation "tp_cmpxchg_suc" constr(j) :=
   iStartProof;
-  with_spec_ctx ltac:(fun _ =>
-      eapply (tac_tp_cmpxchg_suc j);
-        [iSolveTC || fail "tp_cmpxchg_suc: cannot eliminate modality in the goal"
-        |solve_ndisj || fail "tp_cmpxchg_suc: cannot prove 'nclose specN ⊆ ?'"
-        |iAssumptionCore || fail "tp_cmpxchg_suc: cannot find spec_ctx" (* spec_ctx *)
-        |iAssumptionCore || fail "tp_cmpxchg_suc: cannot find '" j " ⤇ ?'"
-        |tp_bind_helper (* e = K'[CmpXchg _ _ _] *)
-        |iSolveTC || fail "tp_cmpxchg_suc: argument is not a value"
-        |iSolveTC || fail "tp_cmpxchg_suc: argument is not a value"
-        |iAssumptionCore || fail "tp_cmpxchg_suc: cannot find '? ↦ ?'"
-        |try (simpl; congruence)     (* v' = v1 *)
-        |try heap_lang.proofmode.solve_vals_compare_safe
-        |simpl; reflexivity || fail "tp_cmpxchg_suc: this should not happen"
-        |pm_reduce (* new goal *)]).
+  eapply (tac_tp_cmpxchg_suc j);
+  [iSolveTC || fail "tp_cmpxchg_suc: cannot eliminate modality in the goal"
+  |solve_ndisj || fail "tp_cmpxchg_suc: cannot prove 'nclose specN ⊆ ?'"
+  |iAssumptionCore || fail "tp_cmpxchg_suc: cannot the RHS '" j "'"
+  |tp_bind_helper (* e = K'[CmpXchg _ _ _] *)
+  |iSolveTC || fail "tp_cmpxchg_suc: argument is not a value"
+  |iSolveTC || fail "tp_cmpxchg_suc: argument is not a value"
+  |iAssumptionCore || fail "tp_cmpxchg_suc: cannot find '? ↦ ?'"
+  |try (simpl; congruence)     (* v' = v1 *)
+  |try heap_lang.proofmode.solve_vals_compare_safe
+  |simpl; reflexivity || fail "tp_cmpxchg_suc: this should not happen"
+  |pm_reduce (* new goal *)].
 
-Lemma tac_tp_faa `{relocG Σ} j Δ1 Δ2 E1 i1 i2 i3 p K' e enew (l : loc)  e2 (z1 z2 : Z) Q :
+Lemma tac_tp_faa `{relocG Σ} k Δ1 Δ2 E1 i1 i2 K' e enew (l : loc)  e2 (z1 z2 : Z) Q :
   (∀ P, ElimModal True false false (|={E1}=> P) P Q Q) →
   nclose specN ⊆ E1 →
-  envs_lookup i1 Δ1 = Some (p, spec_ctx) →
-  envs_lookup_delete false i2 Δ1 = Some (false, j ⤇ e, Δ2)%I →
+  envs_lookup_delete false i1 Δ1 = Some (false, refines_right k e, Δ2)%I →
   e = fill K' (FAA #l e2) →
   IntoVal e2 #z2 →
-  envs_lookup i3 Δ2 = Some (false, l ↦ₛ #z1)%I →
+  envs_lookup i2 Δ2 = Some (false, l ↦ₛ #z1)%I →
   enew = fill K' #z1 →
-  match envs_simple_replace i3 false
-    (Esnoc (Esnoc Enil i2 (j ⤇ enew)) i3 (l ↦ₛ #(z1+z2))%I) Δ2 with
+  match envs_simple_replace i2 false
+    (Esnoc (Esnoc Enil i1 (refines_right k enew)) i2 (l ↦ₛ #(z1+z2))%I) Δ2 with
     | Some Δ3 =>   envs_entails Δ3 Q
     | None => False
   end →
   envs_entails Δ1 Q.
 Proof.
-  rewrite envs_entails_eq. intros ???? -> ?? -> HQ.
-  rewrite -(idemp bi_and (of_envs Δ1)).
-  rewrite {1}(envs_lookup_sound' Δ1 false); last by eassumption.
-  rewrite bi.sep_elim_l.
-  enough (spec_ctx ∗ of_envs Δ1 -∗ Q) as Hq.
-  { rewrite -Hq.
-    destruct p; simpl; last rewrite -(bi.intuitionistic_intuitionistically spec_ctx);
-    rewrite {1}bi.intuitionistically_into_persistently_1 bi.persistently_and_intuitionistically_sep_l;
-    by rewrite (bi.intuitionistic_intuitionistically spec_ctx). }
+  rewrite envs_entails_eq. intros ??? -> ?? -> HQ.
   rewrite envs_lookup_delete_sound //; simpl.
   destruct (envs_simple_replace _ _ _ _) as [Δ3|] eqn:HΔ3; last done.
-  rewrite (envs_simple_replace_sound Δ2 Δ3 i3) //; simpl.
+  rewrite (envs_simple_replace_sound Δ2 Δ3 i2) //; simpl.
   rewrite right_id.
-  (* (S spec_ctx (S (j => fill _ _) (S (l ↦ v) ..))) *)
-  rewrite (assoc _ spec_ctx (j ⤇ fill K' _)%I).
-  (* (S (S spec_ctx (j => fill _ _)) (S (l ↦ v) ..)) *)
-  rewrite assoc.
-  rewrite -(assoc _ spec_ctx (j ⤇ fill K' _)%I).
-  rewrite step_faa //.
+  rewrite /refines_right. rewrite -fill_app.
+  rewrite assoc. rewrite -(assoc _ spec_ctx).
+  rewrite step_faa //. rewrite fill_app.
   rewrite -[Q]elim_modal //.
   apply bi.sep_mono_r.
   apply bi.wand_intro_l.
-  rewrite (comm _ _ (l ↦ₛ _)%I).
+  rewrite (comm _ _ (l ↦ₛ _)%I) assoc.
+  rewrite (comm _ _ (l ↦ₛ _)%I) -assoc.
   rewrite HQ. by apply bi.wand_elim_r.
 Qed.
 
 Tactic Notation "tp_faa" constr(j) :=
   iStartProof;
-  with_spec_ctx ltac:(fun _ =>
-      eapply (tac_tp_faa j);
-          [iSolveTC || fail "tp_faa: cannot eliminate modality in the goal"
-          |solve_ndisj || fail "tp_faa: cannot prove 'nclose specN ⊆ ?'"
-          |iAssumptionCore || fail "tp_faa: cannot find spec_ctx" (* spec_ctx *)
-          |iAssumptionCore || fail "tp_faa: cannot find '" j " ⤇ ?'"
-          |tp_bind_helper (* e = K'[FAA _ _ _] *)
-          |iSolveTC (* IntoVal *)
-          |iAssumptionCore || fail "tp_faa: cannot find '? ↦ ?'"
-          |simpl;reflexivity || fail "tp_faa: this should not happen"
-          |pm_reduce (* new goal *)]).
+  eapply (tac_tp_faa j);
+  [iSolveTC || fail "tp_faa: cannot eliminate modality in the goal"
+  |solve_ndisj || fail "tp_faa: cannot prove 'nclose specN ⊆ ?'"
+  |iAssumptionCore || fail "tp_faa: cannot find the RHS '" j "'"
+  |tp_bind_helper (* e = K'[FAA _ _ _] *)
+  |iSolveTC (* IntoVal *)
+  |iAssumptionCore || fail "tp_faa: cannot find '? ↦ ?'"
+  |simpl;reflexivity || fail "tp_faa: this should not happen"
+  |pm_reduce (* new goal *)].
 
 
-Lemma tac_tp_fork `{relocG Σ} j Δ1 E1 i1 i2 p K' e enew e' Q :
+Lemma tac_tp_fork `{relocG Σ} k Δ1 E1 i1 K' e enew e' Q :
   (∀ P, ElimModal True false false (|={E1}=> P) P Q Q) →
   nclose specN ⊆ E1 →
-  envs_lookup i1 Δ1 = Some (p, spec_ctx) →
-  envs_lookup i2 Δ1 = Some (false, j ⤇ e)%I →
+  envs_lookup i1 Δ1 = Some (false, refines_right k e)%I →
   e = fill K' (Fork e') →
   enew = fill K' #() →
-  match envs_simple_replace i2 false
-      (Esnoc Enil i2 (j ⤇ fill K' #())) Δ1 with
-  | Some Δ2 => envs_entails Δ2 (∀ (j' : nat), j' ⤇ e' -∗ Q)%I
+  match envs_simple_replace i1 false
+      (Esnoc Enil i1 (refines_right k (fill K' #()))) Δ1 with
+  | Some Δ2 => envs_entails Δ2 (∀ k', refines_right k' e' -∗ Q)%I
   | None => False
   end →
   envs_entails Δ1 Q.
 Proof.
-  rewrite envs_entails_eq. intros ????->-> HQ.
-  rewrite -(idemp bi_and (of_envs Δ1)).
-  rewrite {1}(envs_lookup_sound' Δ1 false i1); last by eassumption.
-  rewrite bi.sep_elim_l /=.
-  enough (spec_ctx ∗ of_envs Δ1 -∗ Q) as Hq.
-  { rewrite -Hq.
-    destruct p; simpl; last rewrite -(bi.intuitionistic_intuitionistically spec_ctx);
-    rewrite {1}bi.intuitionistically_into_persistently_1 bi.persistently_and_intuitionistically_sep_l;
-    by rewrite (bi.intuitionistic_intuitionistically spec_ctx). }
+  rewrite envs_entails_eq. intros ???->-> HQ.
   destruct (envs_simple_replace _ _ _ _) as [Δ2|] eqn:HΔ2; last done.
-  rewrite (envs_simple_replace_sound Δ1 Δ2 i2) //; simpl.
+  rewrite (envs_simple_replace_sound Δ1 Δ2 i1) //; simpl.
   rewrite right_id.
-  rewrite (assoc _ spec_ctx (j ⤇ _)%I).
-  rewrite step_fork //.
+  rewrite /refines_right. rewrite -fill_app.
+  rewrite step_fork //. rewrite fill_app.
   rewrite -[Q]elim_modal //.
   apply bi.sep_mono_r.
   apply bi.wand_intro_l.
   rewrite bi.sep_exist_r.
   apply bi.exist_elim. intros j'.
-  rewrite (comm _ (j ⤇ _)%I (j' ⤇ _)%I).
+  (* rewrite (comm _ (j ⤇ _)%I (j' ⤇ _)%I). *)
+  rewrite (comm _ _ (spec_ctx ∗ j' ⤇ e')%I).
   rewrite -assoc.
   rewrite bi.wand_elim_r.
-  rewrite HQ.
-  rewrite (bi.forall_elim j').
+  rewrite HQ. rewrite /refines_right.
+  rewrite (bi.forall_elim (RefId j' [])) /=.
   by rewrite bi.wand_elim_r.
 Qed.
 
 Tactic Notation "tp_fork" constr(j) :=
   iStartProof;
-  with_spec_ctx ltac:(fun _ =>
-      eapply (tac_tp_fork j);
-          [iSolveTC || fail "tp_fork: cannot eliminate modality in the goal"
-          |solve_ndisj || fail "tp_fork: cannot prove 'nclose specN ⊆ ?'"
-          |iAssumptionCore || fail "tp_fork: cannot find spec_ctx" (* spec_ctx *)
-          |iAssumptionCore || fail "tp_fork: cannot find '" j " ⤇ ?'"
-          |tp_bind_helper
-          |simpl; reflexivity || fail "tp_fork: this should not happen"
-          |pm_reduce (* new goal *)]).
+  eapply (tac_tp_fork j);
+  [iSolveTC || fail "tp_fork: cannot eliminate modality in the goal"
+  |solve_ndisj || fail "tp_fork: cannot prove 'nclose specN ⊆ ?'"
+  |iAssumptionCore || fail "tp_fork: cannot find the RHS '" j "'"
+  |tp_bind_helper
+  |simpl; reflexivity || fail "tp_fork: this should not happen"
+  |pm_reduce (* new goal *)].
 
 Tactic Notation "tp_fork" constr(j) "as" ident(j') constr(H) :=
   iStartProof;
-  with_spec_ctx ltac:(fun _ =>
-      eapply (tac_tp_fork j);
-          [iSolveTC || fail "tp_fork: cannot eliminate modality in the goal"
-          |solve_ndisj || fail "tp_fork: cannot prove 'nclose specN ⊆ ?'"
-          |iAssumptionCore || fail "tp_fork: cannot find spec_ctx" (* spec_ctx *)
-          |iAssumptionCore || fail "tp_fork: cannot find '" j " ⤇ ?'"
-          |tp_bind_helper
-          |simpl; reflexivity || fail "tp_fork: this should not happen"
-          |pm_reduce;
-           (iIntros (j') || fail 1 "tp_fork: " j' " not fresh ");
-           (iIntros H || fail 1 "tp_fork: " H " not fresh")
-(* new goal *)]).
+  eapply (tac_tp_fork j);
+  [iSolveTC || fail "tp_fork: cannot eliminate modality in the goal"
+  |solve_ndisj || fail "tp_fork: cannot prove 'nclose specN ⊆ ?'"
+  |iAssumptionCore || fail "tp_fork: cannot find the RHS '" j "'"
+  |tp_bind_helper
+  |simpl; reflexivity || fail "tp_fork: this should not happen"
+  |pm_reduce;
+   (iIntros (j') || fail 1 "tp_fork: " j' " not fresh ");
+   (iIntros H || fail 1 "tp_fork: " H " not fresh")
+(* new goal *)].
 
 Tactic Notation "tp_fork" constr(j) "as" ident(j') :=
   let H := iFresh in tp_fork j as j' H.
 
-Lemma tac_tp_alloc `{relocG Σ} j Δ1 E1 i1 i2 p K' e e' v Q :
+Lemma tac_tp_alloc `{relocG Σ} k Δ1 E1 i1 K' e e' v Q :
   (∀ P, ElimModal True false false (|={E1}=> P) P Q Q) →
   nclose specN ⊆ E1 →
-  envs_lookup i1 Δ1 = Some (p, spec_ctx) →
-  envs_lookup i2 Δ1 = Some (false, j ⤇ e)%I →
+  envs_lookup i1 Δ1 = Some (false, refines_right k e)%I →
   e = fill K' (ref e') →
   IntoVal e' v →
   (* TODO use match here as well *)
   (∀ l : loc, ∃ Δ2,
-    envs_simple_replace i2 false
-       (Esnoc Enil i2 (j ⤇ fill K' #l)) Δ1 = Some Δ2 ∧
+    envs_simple_replace i1 false
+       (Esnoc Enil i1 (refines_right k (fill K' #l))) Δ1 = Some Δ2 ∧
     (envs_entails Δ2 ((l ↦ₛ v) -∗ Q)%I)) →
   envs_entails Δ1 Q.
 Proof.
-  rewrite envs_entails_eq. intros ? ??? Hfill <- HQ.
-  rewrite -(idemp bi_and (of_envs Δ1)).
-  rewrite {1}(envs_lookup_sound' Δ1 false i1); last by eassumption.
-  rewrite bi.sep_elim_l /=.
-  enough (spec_ctx ∗ of_envs Δ1 -∗ Q) as Hq.
-  { rewrite -Hq.
-    destruct p; simpl; last rewrite -(bi.intuitionistic_intuitionistically spec_ctx);
-    rewrite {1}bi.intuitionistically_into_persistently_1 bi.persistently_and_intuitionistically_sep_l;
-    by rewrite (bi.intuitionistic_intuitionistically spec_ctx). }
-  rewrite (envs_lookup_sound' Δ1 false i2); last by eassumption.
-  rewrite Hfill assoc /=.
+  rewrite envs_entails_eq. intros ??? Hfill <- HQ.
+  rewrite (envs_lookup_sound' Δ1 false i1); last by eassumption.
+  rewrite /refines_right.
+  rewrite Hfill -fill_app /=.
   rewrite step_alloc //.
   rewrite -[Q]elim_modal //.
   apply bi.sep_mono_r, bi.wand_intro_l.
   rewrite bi.sep_exist_r.
   apply bi.exist_elim=> l.
   destruct (HQ l) as (Δ2 & HΔ2 & HQ').
-  rewrite (envs_simple_replace_sound' _ _ i2 _ _ HΔ2).
-  rewrite (comm _ (j ⤇ _)%I (l ↦ₛ _)%I).
-  rewrite -assoc /= right_id.
+  rewrite (envs_simple_replace_sound' _ _ i1 _ _ HΔ2) /=.
+  rewrite HQ' right_id.
+  rewrite /refines_right fill_app.
+  rewrite (comm _ _ (l ↦ₛ _)%I).
+  rewrite assoc.
+  rewrite (comm _ _ (l ↦ₛ _)%I).
+  rewrite -(assoc _ (l ↦ₛ _)%I spec_ctx _). rewrite -assoc.
   rewrite bi.wand_elim_r.
-  rewrite HQ'.
   by rewrite bi.wand_elim_r.
 Qed.
 
@@ -578,97 +494,95 @@ Tactic Notation "tp_alloc" constr(j) "as" ident(l) constr(H) :=
         [ reduction.pm_reflexivity
         | (iIntros H; tp_normalise j) || fail 1 "tp_alloc:" H "not correct intro pattern" ] in
   iStartProof;
-  with_spec_ctx ltac:(fun _ =>
-      eapply (tac_tp_alloc j);
-        [iSolveTC || fail "tp_alloc: cannot eliminate modality in the goal"
-        |solve_ndisj || fail "tp_alloc: cannot prove 'nclose specN ⊆ ?'"
-        |iAssumptionCore || fail "tp_alloc: cannot find spec_ctx" (* spec_ctx *)
-        |iAssumptionCore || fail "tp_alloc: cannot find '" j " ⤇ ?'"
-        |tp_bind_helper
-        |iSolveTC || fail "tp_alloc: expressions is not a value"
-        |finish ()
-(* new goal *)]).
+  eapply (tac_tp_alloc j);
+  [iSolveTC || fail "tp_alloc: cannot eliminate modality in the goal"
+  |solve_ndisj || fail "tp_alloc: cannot prove 'nclose specN ⊆ ?'"
+  |iAssumptionCore || fail "tp_alloc: cannot find the RHS '" j "'"
+  |tp_bind_helper
+  |iSolveTC || fail "tp_alloc: expressions is not a value"
+  |finish ()
+(* new goal *)].
 
 Tactic Notation "tp_alloc" constr(j) "as" ident(j') :=
   let H := iFresh in tp_alloc j as j' H.
 
 
-(*
-(**************************)
-(* tp_apply *)
+(* *)
+(* (**************************) *)
+(* (* tp_apply *) *)
 
-Fixpoint print_sel (ss : list sel_pat) (s : string) :=
-  match ss with
-  | nil => s
-  | SelPure :: ss' => (String "%" (String " " (print_sel ss' s)))
-  | SelPersistent :: ss' =>  (String "#" (print_sel ss' s))
-  | SelSpatial :: ss' => (* no clue :( *) (print_sel ss' s)
-  | SelIdent (INamed n) :: ss' => append n (String " " (print_sel ss' s))
-  | SelIdent (IAnon _) :: ss' => String "?" (String " " (print_sel ss' s))
-  (* wat to do with the index? *)
-  end.
+(* Fixpoint print_sel (ss : list sel_pat) (s : string) := *)
+(*   match ss with *)
+(*   | nil => s *)
+(*   | SelPure :: ss' => (String "%" (String " " (print_sel ss' s))) *)
+(*   | SelPersistent :: ss' =>  (String "#" (print_sel ss' s)) *)
+(*   | SelSpatial :: ss' => (* no clue :( *) (print_sel ss' s) *)
+(*   | SelIdent (INamed n) :: ss' => append n (String " " (print_sel ss' s)) *)
+(*   | SelIdent (IAnon _) :: ss' => String "?" (String " " (print_sel ss' s)) *)
+(*   (* wat to do with the index? *) *)
+(*   end. *)
 
-Ltac print_sel ss :=
-  lazymatch type of ss with
-  | list sel_pat => eval vm_compute in (print_sel ss "")
-  | string => ss
-  end.
+(* Ltac print_sel ss := *)
+(*   lazymatch type of ss with *)
+(*   | list sel_pat => eval vm_compute in (print_sel ss "") *)
+(*   | string => ss *)
+(*   end. *)
 
-Definition appP (ss : option (list sel_pat)) (Hj Hs : string) :=
-  match ss with
-  | Some ss' => cons (SelIdent Hs) (app ss' [SelIdent Hj])
-  | None => cons (SelIdent Hs) [SelIdent Hj]
-  end.
+(* Definition appP (ss : option (list sel_pat)) (Hj Hs : string) := *)
+(*   match ss with *)
+(*   | Some ss' => cons (SelIdent Hs) (app ss' [SelIdent Hj]) *)
+(*   | None => cons (SelIdent Hs) [SelIdent Hj] *)
+(*   end. *)
 
-Definition add_elim_pat (pat : string) (Hj : string) :=
-  match pat with
-  | EmptyString => Hj
-  | _ => append (String "[" (append Hj (String " " pat))) "]"
-  end.
+(* Definition add_elim_pat (pat : string) (Hj : string) := *)
+(*   match pat with *)
+(*   | EmptyString => Hj *)
+(*   | _ => append (String "[" (append Hj (String " " pat))) "]" *)
+(*   end. *)
 
-Tactic Notation "tp_apply" constr(j) open_constr(lem) "with" constr(Hs) "as" constr(Hr) :=
-  iStartProof;
-  let rec find Γ j :=
-    match Γ with
-    | Esnoc ?Γ (IAnon _) ?P =>
-      find Γ j
-    | Esnoc ?Γ (INamed ?Hj) ?P =>
-      lazymatch P with
-      | (j ⤇ _)%I => Hj
-      | _ => find Γ j
-      end
-    | Enil => fail 2 "tp_apply: cannot find " j " ⤇ _ "
-    | _ => fail 2 "tp_apply: unknown error in find"
-    end in
-  let rec findSpec Γp Γs :=
-    match Γp with
-    | Esnoc ?Γ (IAnon _) _ => findSpec Γ Γs
-    | Esnoc ?Γ (INamed ?Hspec) ?P =>
-      lazymatch P with
-      | (spec_ctx _)%I => Hspec
-      | _ => findSpec Γ Γs
-      end
-    | Enil =>
-      match Γs with
-      | Enil => fail 2 "tp_apply: cannot find spec_ctx _"
-      | _ => findSpec Γs Enil
-      end
-    | _ => fail 2 "tp_apply: unknown error in findSpec"
-    end in
-  match goal with
-  | |- envs_entails (Envs ?Γp ?Γs) ?Q =>
-    let Hj := (find Γs j) in
-    let Hspec := findSpec Γp Γs in
-    let pat := eval vm_compute in (appP (sel_pat.parse Hs) Hj Hspec) in
-    let pats := print_sel pat in
-    let elim_pats := eval vm_compute in (add_elim_pat Hr Hj) in
-    iMod (lem with pats) as elim_pats; first try by solve_ndisj
-  | _ => fail "tp_apply: cannot parse the context"
-  end.
+(* Tactic Notation "tp_apply" constr(j) open_constr(lem) "with" constr(Hs) "as" constr(Hr) := *)
+(*   iStartProof; *)
+(*   let rec find Γ j := *)
+(*     match Γ with *)
+(*     | Esnoc ?Γ (IAnon _) ?P => *)
+(*       find Γ j *)
+(*     | Esnoc ?Γ (INamed ?Hj) ?P => *)
+(*       lazymatch P with *)
+(*       | (j ⤇ _)%I => Hj *)
+(*       | _ => find Γ j *)
+(*       end *)
+(*     | Enil => fail 2 "tp_apply: cannot find " j " ⤇ _ " *)
+(*     | _ => fail 2 "tp_apply: unknown error in find" *)
+(*     end in *)
+(*   let rec findSpec Γp Γs := *)
+(*     match Γp with *)
+(*     | Esnoc ?Γ (IAnon _) _ => findSpec Γ Γs *)
+(*     | Esnoc ?Γ (INamed ?Hspec) ?P => *)
+(*       lazymatch P with *)
+(*       | (spec_ctx _)%I => Hspec *)
+(*       | _ => findSpec Γ Γs *)
+(*       end *)
+(*     | Enil => *)
+(*       match Γs with *)
+(*       | Enil => fail 2 "tp_apply: cannot find spec_ctx _" *)
+(*       | _ => findSpec Γs Enil *)
+(*       end *)
+(*     | _ => fail 2 "tp_apply: unknown error in findSpec" *)
+(*     end in *)
+(*   match goal with *)
+(*   | |- envs_entails (Envs ?Γp ?Γs) ?Q => *)
+(*     let Hj := (find Γs j) in *)
+(*     let Hspec := findSpec Γp Γs in *)
+(*     let pat := eval vm_compute in (appP (sel_pat.parse Hs) Hj Hspec) in *)
+(*     let pats := print_sel pat in *)
+(*     let elim_pats := eval vm_compute in (add_elim_pat Hr Hj) in *)
+(*     iMod (lem with pats) as elim_pats; first try by solve_ndisj *)
+(*   | _ => fail "tp_apply: cannot parse the context" *)
+(*   end. *)
 
-Tactic Notation "tp_apply" constr(j) open_constr(lem) "with" constr(Hs) := tp_apply j lem with Hs as "".
+(* Tactic Notation "tp_apply" constr(j) open_constr(lem) "with" constr(Hs) := tp_apply j lem with Hs as "". *)
 
-Tactic Notation "tp_apply" constr(j) open_constr(lem) "as" constr(Hr) := tp_apply j lem with "" as Hr.
+(* Tactic Notation "tp_apply" constr(j) open_constr(lem) "as" constr(Hr) := tp_apply j lem with "" as Hr. *)
 
-Tactic Notation "tp_apply" constr(j) open_constr(lem) := tp_apply j lem with "" as "".
-*)
+(* Tactic Notation "tp_apply" constr(j) open_constr(lem) := tp_apply j lem with "" as "". *)
+(* *)
